Games/games/Chomp.lean
@@ -7,6 +7,7 @@ Author: Yves Jäckle.
 import Games.exLib.Nat
 import Games.gameLib.Basic
 import Mathlib.Tactic
+import Mathlib.Data.List.ProdSigma
 
 
 def domi (p q : ℕ × ℕ) : Prop := p.1 ≤ q.1 ∧ p.2 ≤ q.2
@@ -28,20 +29,6 @@ instance : DecidableRel nondomi :=
 
 variable {height length : ℕ}
 
-structure Chomp_law (hist : List (ℕ × ℕ)) (act : ℕ × ℕ) : Prop where
-  h : act.2 ≤ height
-  l : act.1 ≤ length
-  nd : ∀ q ∈ hist, nondomi q act
-
-/--
-State is basicly hist : it collects the places where a player has chomped
-the board. Initially, nothing was chomped. We transition by adding moves.
--/
-def Chomp : Symm_Game_World (List (ℕ × ℕ)) (ℕ × ℕ) where
-  init_game_state := []
-  win_states := (fun l => ∀ p : ℕ × ℕ, (∀ q ∈ l, nondomi q p) → p = (0,0))
-  transition := fun h a => a :: h
-  law := @Chomp_law height length
 
 
 instance (l : List (ℕ × ℕ)) : DecidablePred (fun p => ∀ q ∈ l, nondomi q p) :=
@@ -52,5 +39,95 @@ instance (l : List (ℕ × ℕ)) : DecidablePred (fun p => ∀ q ∈ l, nondomi 
 
 -- pretty print the state
 def pp_Chomp_state (l : List (ℕ × ℕ)) :=
-  (List.product (List.range (length +1)) (List.range (height +1))).filter
+  ((List.range (length + 1)) ×ˢ (List.range (height + 1))).filter
     (fun p => ∀ q ∈ l, nondomi q p)
+
+
+structure Chomp_law (hist : List (ℕ × ℕ)) (act : ℕ × ℕ) : Prop where
+  h : act.2 ≤ height
+  l : act.1 ≤ length
+  nd : @pp_Chomp_state height length hist ≠ [(0,0)] → ∀ q ∈ hist, nondomi q act
+  nz : act ≠ (0,0) -- even when end is reached, the partial function phenomenon forbids playing (0,0)
+  -- for the game to be playable, one of `height` or `length` must be positive
+
+def Chomp : Symm_Game_World (List (ℕ × ℕ)) (ℕ × ℕ) where
+  init_game_state := (@pp_Chomp_state height length) []
+  win_states := (fun state => state = [(0,0)])
+  transition := fun hist act => (@pp_Chomp_state height length) (act :: hist)
+  law := @Chomp_law height length
+
+
+
+def Chomp_measure (hist : List (ℕ × ℕ)) : ℕ :=
+  (List.length (@pp_Chomp_state height length hist))
+
+
+
+lemma Chomp_measure_decrease
+  (f_strat s_strat : Strategy (List (ℕ × ℕ)) (ℕ × ℕ))
+  (f_law : Strategy_legal (@Chomp height length).init_game_state (fun _ => (@Chomp height length).law) f_strat s_strat f_strat)
+  (s_law : Strategy_legal (@Chomp height length).init_game_state (fun _ => (@Chomp height length).law) f_strat s_strat s_strat) :
+  let H := History_on_turn (@Chomp height length).init_game_state f_strat s_strat
+  ∀ turn : ℕ, ((@Chomp_measure height length) (H (turn + 1)) < (@Chomp_measure height length) (H (turn))) ∨ ((@Chomp_measure height length) (H (turn +1)) = 0) :=
+  by
+  sorry
+
+
+lemma Chomp_measure_lb
+  (hg : 1 ≤ height ∨ 1 ≤ length)
+  (f_strat s_strat : Strategy (List (ℕ × ℕ)) (ℕ × ℕ))
+  (f_law : Strategy_legal (@Chomp height length).init_game_state (fun _ => (@Chomp height length).law) f_strat s_strat f_strat)
+  (s_law : Strategy_legal (@Chomp height length).init_game_state (fun _ => (@Chomp height length).law) f_strat s_strat s_strat)
+  (turn : ℕ) :
+  let H := History_on_turn (@Chomp height length).init_game_state f_strat s_strat
+  1 ≤ (@Chomp_measure height length) (H turn) :=
+  by
+  intro H
+  dsimp [Strategy_legal, Chomp] at *
+  specialize f_law turn
+  specialize s_law turn
+  rw [Nat.one_le_iff_ne_zero]
+  intro con
+  rw [Chomp_measure, List.length_eq_zero, pp_Chomp_state, List.filter_eq_nil] at con
+  specialize con (0,0) (by rw [List.mem_product] ; constructor <;> {rw [List.mem_range] ; apply Nat.zero_lt_succ})
+  apply con
+  apply decide_eq_true
+  intro q qH
+  rw [nondomi,domi]
+  push_neg
+  dsimp
+  intro fz
+  rw [Nat.le_zero] at fz
+  by_contra! sz
+  rw [Nat.le_zero] at sz
+  -- do a cases on turn ; the zero case is absurd with qH
+  -- use Symm_Game_World.mem_History_on_turn at qH
+  -- then derive a contradiction with Chomp_law.nz for each case
+
+
+#exit
+
+
+lemma Chomp_termination_pre
+  (f_strat s_strat : Strategy (List (ℕ × ℕ)) (ℕ × ℕ))
+  (f_law : Strategy_legal (@Chomp height length).init_game_state (fun _ => (@Chomp height length).law) f_strat s_strat f_strat)
+  (s_law : Strategy_legal (@Chomp height length).init_game_state (fun _ => (@Chomp height length).law) f_strat s_strat s_strat) :
+  let H := History_on_turn (@Chomp height length).init_game_state f_strat s_strat
+  ∃ turn : ℕ, (@Chomp_measure height length) (H turn) = 1 :=
+  by
+  intro h
+  apply Nat.well_ordered
+  have := Chomp_measure_decrease f_strat s_strat f_law s_law
+  dsimp at *
+  apply this
+
+lemma Chomp_measure_lowest_iff
+  (hg : 1 ≤ height ∨ 1 ≤ length)
+  (f_strat s_strat : Strategy (List (ℕ × ℕ)) (ℕ × ℕ))
+  (f_law : Strategy_legal (@Chomp height length).init_game_state (fun _ => (@Chomp height length).law) f_strat s_strat f_strat)
+  (s_law : Strategy_legal (@Chomp height length).init_game_state (fun _ => (@Chomp height length).law) f_strat s_strat s_strat)
+  (turn : ℕ) :
+  let H := History_on_turn (@Chomp height length).init_game_state f_strat s_strat
+  (@Chomp_measure height length) (H turn) = 1 ↔ (@Chomp height length).win_states (H turn) :=
+  by
+  sorry
