Games/gameLib/Termination_CounterExample.lean
@@ -4,9 +4,16 @@ Released under Apache 2.0 license as described in the file LICENSE.
 Author: Yves Jäckle.
 -/
 
-import Games.gameLib.Basic
+import Games.games.Chomp
 import Mathlib.Tactic
 
+
+
+def InfiChomp : Symm_Game_World (List (ℕ × ℕ)) (ℕ × ℕ) where
+  init_game_state := []
+  win_states := (fun l => ∀ p : ℕ × ℕ, (∀ q ∈ l, nondomi q p) → p = (0,0))
+  transition := fun h a => a :: h
+  law := fun hist act => ∀ q ∈ hist, nondomi q act
 
 -- infinite chomp ; we may find aribrtarily long games
 example : ∃ α β : Type, ∃ g : Symm_Game_World α β,
